Minor changes

ref_impl/src/verifier/testing/testing_collect_expressions.ts
@@ -3,7 +3,6 @@
 // Licensed under the MIT license. See LICENSE.txt file in the project root for full license information.
 //-------------------------------------------------------------------------------------------------------
 
-import * as FS from "fs";
 import { sanitizeName, bosqueToInvokeDecl } from "../util"
 import { TranslatorBosqueFStar, FStarDeclaration } from "../translator_bosque_fstar";
 
@@ -13,21 +12,19 @@ setImmediate(() => {
     // Windows Machine
     const directory = "/Users/t-jocast/code/BosqueLanguage/ref_impl/src/test/apps/max/";
     const fileName = "main.bsq";
-    const mapDeclarations = bosqueToInvokeDecl({ directory: directory, fileName: fileName });
     const fkey = "NSMain::main";
+
+    const mapDeclarations = bosqueToInvokeDecl({ directory: directory, fileName: fileName }); 
     let fstarFileName = (sanitizeName(fkey) + "_" + fileName).replace("bsq", "fst");
     fstarFileName = fstarFileName.charAt(0).toUpperCase() + fstarFileName.slice(1);
-    
-    const fd = FS.openSync(fstarFileName, 'w');
-    FS.writeSync(fd, `module ${fstarFileName.slice(0, -4)}\n\n`);
 
-    const translation = new TranslatorBosqueFStar(mapDeclarations);
+    const translation = new TranslatorBosqueFStar(mapDeclarations, fstarFileName);
     const fstarStackProgram = translation.collectExpr(fkey);
+
     fstarStackProgram.reverse();
+    translation.printPrelude();
     while (fstarStackProgram.length > 0) {
-        const currentDeclaration = fstarStackProgram.pop() as FStarDeclaration;
-        FS.writeSync(fd, currentDeclaration.printVal());
-        FS.writeSync(fd, currentDeclaration.printLet());
+        (fstarStackProgram.pop() as FStarDeclaration).print(translation.fd);
     }
-    FS.closeSync(fd);
+    translation.closeFS();
 });
