ref_impl/NSMain__main_main.fst
@@ -14,13 +14,28 @@ let nSMain__max0 x y =
                     let _return_ = _ir_ret__2 in 
                         _return_
 
+val nSMain__max0 : int -> int -> Tot int
+let nSMain__max0 x y = 
+    let __tmp_0 = (op_GreaterThanOrEqual x y) in 
+        if (op_Equality __tmp_0 true) then 
+            let _ir_ret__1 = x in 
+                let _ir_ret__2 = _ir_ret__1 in 
+                    let _return_ = _ir_ret__2 in 
+                        _return_
+        else 
+            let _ir_ret_ = y in 
+                let _ir_ret__2 = _ir_ret_ in 
+                    let _return_ = _ir_ret__2 in 
+                        _return_
+
 val nSMain__main : int
 let nSMain__main  = 
     let x = 10 in 
         let y = 20 in 
-            let __tmp_2 = (nSMain__max0 x y) in 
-                let z = __tmp_2 in 
-                    let _ir_ret_ = z in 
-                        let _return_ = _ir_ret_ in 
-                            _return_
+            let __tmp_3 = (nSMain__max0 x y) in 
+                let __tmp_2 = (nSMain__max0 __tmp_3 y) in 
+                    let z = __tmp_2 in 
+                        let _ir_ret_ = z in 
+                            let _return_ = _ir_ret_ in 
+                                _return_
 
